code/ecdsap256/Hacl.Impl.P256.Compression.fst
@@ -8,7 +8,6 @@ module ST = FStar.HyperStack.ST
 open Lib.IntTypes
 open Lib.Buffer
 
-open Hacl.Spec.P256.Bignum
 open Hacl.Impl.P256.Bignum
 open Hacl.Impl.P256.Field
 module P = Hacl.Impl.P256.Point
