code/ecdsap256/Hacl.Impl.P256.Core.fst
@@ -8,9 +8,8 @@ module ST = FStar.HyperStack.ST
 open Lib.IntTypes
 open Lib.Buffer
 
-open Hacl.Spec.P256.Bignum
-open Hacl.Impl.P256.SolinasReduction
 open Hacl.Impl.P256.Bignum
+open Hacl.Impl.P256.SolinasReduction
 
 module S = Spec.P256
 module SM = Hacl.Spec.P256.MontgomeryMultiplication
