code/ecdsap256/Hacl.Impl.P256.Field.fsti
@@ -8,7 +8,7 @@ module ST = FStar.HyperStack.ST
 open Lib.IntTypes
 open Lib.Buffer
 
-open Hacl.Spec.P256.Bignum
+open Hacl.Impl.P256.Bignum
 
 module S = Spec.P256
 module SM = Hacl.Spec.P256.MontgomeryMultiplication
